Create Lib.Array, Lib.Maths and TreeSync.Lemmas

fstar/new/TreeSync.fst
@@ -1,5 +1,8 @@
 module TreeSync
 
+open Lib.Array
+open Lib.Maths
+
 
 (* Base datatypes *)
 type bytes_t = Seq.seq nat
@@ -13,86 +16,28 @@ let datatype_t = eqtype
 let sign_key_t = bytes_t
 let verif_key_t = bytes_t
 
+let enc_key_t = bytes_t
+let dec_key_t = bytes_t
 
-(* Datastructures *)
-let array a = Seq.seq a
-let length a = Seq.length a
-let empty = Seq.empty
-let singleton x = Seq.create 1 x
-let append x y = Seq.append x y
-
-(* Infix operators *)
-let op_String_Access x y = Seq.index x y
-let op_String_Assignment x y z = Seq.upd x y z
-
-(* Datastructures operators *)
-let rec mapi (f:'a -> 'b) (x:array 'a) (i:nat{i <= length x}) : y:array 'b{length y = i} =
-  if i = 0 then empty else Seq.snoc (mapi f x (i-1)) (f x.[i-1])
-
-let map (f:'a -> 'b) (x:array 'a) = mapi f x (length x)
-
-
-val lemma_singleton: x:array 'a{length x = 1} -> i:nat{i<length x} ->
-  Lemma (singleton x.[i] == x)
-	[SMTPat (singleton x.[i])]
-let lemma_singleton x i = Seq.lemma_eq_intro (singleton x.[i]) x
-
-val lemma_map_singleton: f:('a -> 'b) -> x:array 'a{length x = 1} ->
-    Lemma (singleton (f (x.[0])) == map f x)
-	  [SMTPatOr [
-	    [SMTPat (singleton (f (x.[0])));
-	     SMTPat (map f x)]]]
-let lemma_map_singleton f x = admit()
-
-val lemma_map_append: f:('a -> 'b) -> x:array 'a -> y:array 'a ->
-    Lemma (append (map f x) (map f y) == map f (append x y))
-	  [SMTPatOr [
-	    [SMTPat (append (map f x) (map f y));
-	     SMTPat (map f (append x y))]]]
-let lemma_map_append f x y = admit()
-
-
-let sub (x:array 'a) (i:nat{i < length x}) (l:nat{i+l <= length x}) = Seq.slice x i (i+l)
-
-let split (x:array 'a) (i:nat{i < length x}): res:(array 'a * array 'a){let (y,z) = res in x == append y z /\ length y = i} =
-  let s1 = sub x 0 i in
-  let s2 = sub x i (length x - i) in
-  Seq.lemma_eq_intro x (append s1 s2);
-  (s1,s2)
-
-
-let rec foldi (f:'a -> 'b -> 'a) (x:array 'b) (init:'a) (n:nat{n <= length x}) =
-  if n = 0 then init
-  else f (foldi f x init (n-1)) x.[n-1]
-
-val fold: f:('a -> 'b -> 'a) -> array 'b -> 'a -> 'a
-let fold f x a = foldi f x a (length x)
-
-
-type principal_t = string
 
 (* Identity and Credentials *)
+type principal_t = string
+
 type credential_t: eqtype = {
   cred_name: principal_t;
-  cred_sid: nat;
+  cred_issuer: principal_t;
   cred_version: nat;
   cred_identity_key: verif_key_t;
-  cred_issuer: principal_t;
   cred_signature: bytes_t;
+  cred_enc_key: enc_key_t;
 }
 
-val name: credential_t -> string
-let name c = c.cred_name
 
-val identity_key: credential_t -> verif_key_t
-let identity_key c = c.cred_identity_key
-
-assume val validate_: credential_t -> bool
+assume val validate_credential: credential_t -> bool
 
 val valid_credential_p: credential_t -> pred_p
-let valid_credential_p c = validate_ c
+let valid_credential_p c = validate_credential c
 
-(* Secrets associated to a leaf *)
 
 
 type direction_t = | Left | Right
@@ -109,15 +54,29 @@ type leaf_secrets_t: eqtype = {
 
 (* Public Information about a Group Member *)
 type leaf_package_t = {
-  leaf_version: nat;
   leaf_credential: credential_t;
+  leaf_version: nat;
+  leaf_content: bytes_t;
 }
 
+let initial_leaf_package_p (olp:option leaf_package_t) =
+  match olp with
+  | None -> True
+  | Some lp -> valid_credential_p lp.leaf_credential /\ lp.leaf_version = 0
+
+let mk_initial_leaf_package (c:credential_t) =
+  { leaf_credential = c;
+    leaf_version = 0;
+    leaf_content = empty_bytes;}
+
+
 type node_package_t = {
-  node_from : direction_t;
+  node_version: nat;
   node_content: bytes_t
 }
 
+
+(* Tree and Paths definitions*)
 type tree_t (lev:nat) =
  | Leaf: actor:credential_t{lev=0} -> olp:option leaf_package_t -> tree_t lev
  | Node: actor:credential_t{lev>0} -> onp:option node_package_t ->
@@ -128,76 +87,73 @@ type path_t (lev:nat) =
  | PNode: onp:option node_package_t{lev>0} ->
 	       next:path_t (lev-1) -> path_t lev
 
+
+(* TreeSync state and accessors*)
 type state_t: eqtype = {
   st_group_id: nat;
   st_levels: nat;
   st_tree: tree_t st_levels;
-  st_epoch: nat;
-  st_transcript_hash: bytes_t;
+  st_version: nat;
+  st_transcript: bytes_t;
 }
 
-let index_n (l:nat) = x:nat{x < pow2 l}
-let level_n = n:nat{pow2 n < pow2 32}
+type index_n (l:nat) = x:nat{x < pow2 l}
+type level_n = n:nat{pow2 n < pow2 32}
 
-let group_id g = g.st_group_id
-let max_size g = pow2 g.st_levels
-let epoch g = g.st_epoch
+val group_id: state_t -> nat
+let group_id st = st.st_group_id
 
+val max_size: state_t -> nat
+let max_size st = pow2 st.st_levels
 
-(* Group State Data Structure *)
-(* val state_t: datatype_t *)
-(* val group_id: state_t -> nat *)
-(* val max_size: state_t -> nat *)
-(* val epoch: state_t -> nat *)
+val epoch: state_t -> nat
+let epoch st = st.st_version
 
-type index_t (g:state_t) = i:nat{i < max_size g}
-
-type member_array_t (sz:nat) = a:array (option leaf_package_t){length a = sz}
+type index_t (st:state_t) = i:nat{i < max_size st}
 
 
+
+(* Membership *)
+type member_array_t (sz:nat) = a:array (option credential_t){length a = sz}
 
 let rec membership_tree (l:nat) (t:tree_t l): member_array_t (pow2 l) =
   match t with
-  | Leaf _ mi -> singleton mi
+  | Leaf _ olp ->
+    (match olp with
+    | None -> singleton None
+    | Some lp -> singleton (Some lp.leaf_credential))
   | Node _ _ left right -> append (membership_tree (l-1) left)
 				 (membership_tree (l-1) right)
 
-val membership: g:state_t -> member_array_t (max_size g)
-let membership g = membership_tree g.st_levels g.st_tree
 
-val log2: sz:pos -> option nat
-let rec log2 sz =
-  if sz = 1 then Some 0
-  else if sz % 2 = 1 then None
-       else match log2 (sz/2) with
-	    | None -> None
-	    | Some l -> Some (1+l)
+val membership: st:state_t -> member_array_t (max_size st)
+let membership st = membership_tree st.st_levels st.st_tree
 
-let rec log2_lemma (sz:pos):
-  Lemma (match log2 sz with
-	 | None -> True
-	 | Some l -> sz == pow2 l)
-	 [SMTPat (log2 sz)] =
-   if sz = 1 then ()
-   else log2_lemma (sz/2)
 
-val create_tree: l:nat -> c:credential_t ->
-		 init:member_array_t (pow2 l) ->
-		 t:tree_t l{membership_tree l t == init}
-
-(* Create a new tree from a member array *)
-let rec create_tree (l:nat) (c:credential_t) (init:member_array_t (pow2 l)) =
-  if l = 0 then Leaf c init.[0]
-  else let init_l,init_r = split init (pow2 (l-1)) in
-    let left = create_tree (l-1) c init_l in
-    let right = create_tree (l-1) c init_r in
-    Node c None left right
 
 (* Auxiliary tree functions *)
 let child_index (l:pos) (i:index_n l) : index_n (l-1) & direction_t =
   if i < pow2 (l - 1) then (i, Left) else (i-pow2 (l-1), Right)
 
 let order_subtrees dir (l,r) = if dir = Left then (l,r) else (r,l)
+
+
+
+(* Create a new tree from a member array *)
+val create_tree: l:nat -> actor:credential_t ->
+		 init:member_array_t (pow2 l) ->
+		 t:tree_t l{membership_tree l t == init}
+
+let rec create_tree (l:nat) (actor:credential_t) (init:member_array_t (pow2 l)) =
+  if l = 0 then
+    match init.[0] with
+    | None -> Leaf actor None
+    | Some c -> Leaf actor (Some (mk_initial_leaf_package c))
+  else
+    let init_l,init_r = split init (pow2 (l-1)) in
+    let left = create_tree (l-1) actor init_l in
+    let right = create_tree (l-1) actor init_r in
+    Node actor None left right
 
 (* Apply a path to a tree *)
 let rec apply_path (l:nat) (i:nat{i<pow2 l}) (a:credential_t)
@@ -210,190 +166,102 @@ let rec apply_path (l:nat) (i:nat{i<pow2 l}) (a:credential_t)
      then Node a onp (apply_path (l-1) j a left next) right
      else Node a onp left (apply_path (l-1) j a right next)
 
+
 (* Create a blank path after modifying a leaf *)
-let rec blank_path (l:nat) (i:index_n l) (olp:option leaf_package_t) : path_t l =
-  if l = 0 then PLeaf olp
+let rec blank_path (l:nat) (i:index_n l) (oc:option credential_t) : path_t l =
+  if l = 0 then
+    match oc with
+    | None -> PLeaf None
+    | Some c -> PLeaf (Some (mk_initial_leaf_package c))
   else let (j,dir) = child_index l i in
-    PNode None (blank_path (l-1) j olp)
-
-let rec blank_path_lemma (l:nat) (i:index_n l) (olp:option leaf_package_t) (a:credential_t) (t:tree_t l) :
-                    Lemma (let t' = apply_path l i a t (blank_path l i olp) in
-                          membership_tree l t' == ((membership_tree l t).[i] <- olp)) =
-    match t with
-    | Leaf _ _ ->
-	   let t' = apply_path l i a t (blank_path l i olp) in
-	   Seq.lemma_eq_intro (membership_tree l t') ((membership_tree l t).[i] <- olp)
-    | Node _ _ left right ->
-      let (j,dir) = child_index l i in
-      let (child,sibling) = order_subtrees dir (left,right) in
-      let p = PNode None (blank_path (l-1) j olp) in
-      blank_path_lemma (l-1) j olp a child;
-      let t' = apply_path l i a t (blank_path l i olp) in
-      Seq.lemma_eq_intro (membership_tree l t') ((membership_tree l t).[i] <- olp)
-
-let initial_leaf_package (olp:option leaf_package_t) =
-  match olp with
-  | None -> True
-  | Some lp -> valid_credential_p lp.leaf_credential /\ lp.leaf_version = 0
-
-(* Create an update path from a leaf to the root *)
-let rec update_path (l:nat) (t:tree_t l) (i:nat{i<pow2 l}) (lp_i:leaf_package_t) : option (path_t l) =
-  match t with
-  | Leaf _ None -> None
-  | Leaf _ (Some mi) -> if name(mi.leaf_credential) = name(lp_i.leaf_credential)
-                       then Some (PLeaf (Some lp_i))
-                       else None
-  | Node _ _ left right ->
-     let (j,dir) = child_index l i in
-     let (child,sibling) = order_subtrees dir (left,right) in
-     match update_path (l-1) child j lp_i with
-       | None -> None
-       | Some next ->
-         let np = {node_from = dir; node_content = empty_bytes} in // BB. TODO.
-         Some (PNode (Some np) next)
-
-let rec update_path_lemma (l:nat) (i:nat{i<pow2 l}) (a:credential_t) (t:tree_t l) (lp_i:leaf_package_t):
-  Lemma (match update_path l t i lp_i with
-		  | None -> True
-		  | Some p ->
-			 (match (membership_tree l t).[i] with
-			 | None -> False
-			 | Some mi_old -> name(mi_old.leaf_credential) == name(lp_i.leaf_credential) /\
-					           (let t' = apply_path l i a t p in
-					           membership_tree l t' = ((membership_tree l t).[i] <- Some lp_i)))) =
-   match t with
-   | Leaf _ None -> ()
-   | Leaf _ (Some mi) ->
-     if name(mi.leaf_credential) = name(lp_i.leaf_credential)
-     then let p : path_t l = PLeaf (Some lp_i) in
-	  let t' = apply_path l i a t p in
-	  Seq.lemma_eq_intro (membership_tree l t')
-	                     ((membership_tree l t).[i] <- Some lp_i)
-     else ()
-  | Node _ _ left right ->
-     let (j,dir) = child_index l i in
-     let (child,sibling) = order_subtrees dir (left,right) in
-     match update_path (l-1) child j lp_i with
-       | None -> ()
-       | Some next ->
-         update_path_lemma (l-1) j a child lp_i;
-         let np = {node_from = dir; node_content = empty_bytes} in // BB. TODO.
-         let p = PNode (Some np) next in
-	      let t' = apply_path l i a t p in
-	      Seq.lemma_eq_intro (membership_tree l t')
-		                      ((membership_tree l t).[i] <- Some lp_i)
+    PNode None (blank_path (l-1) j oc)
 
 
-assume val hash_state: state_t -> bytes_t
+///
+/// API
+///
+
+(* Operations on the state *)
+type operation_t: eqtype = {
+  op_level: nat;
+  op_index: index_n op_level;
+  op_actor: credential_t;
+  op_path: path_t op_level;
+}
+
+(* Create an operation that modifies the group state *)
+val mk_operation: st:state_t -> actor:credential_t
+  -> i:index_t st -> p:path_t st.st_levels
+  -> Tot (option operation_t)
+
+let mk_operation st actor i p = admit()
 
 
 (* Create a new group state *)
 val create: gid:nat -> sz:pos -> init:member_array_t sz
-          -> entropy:bytes_t	-> option state_t
+  -> Tot (option state_t)
 
-let create gid sz init leaf_secret =
+let create gid sz init =
   match init.[0], log2 sz with
-  | None,_ -> None
-  | _,None -> None
-  | Some c,Some l ->
-    let t = create_tree l c.leaf_credential init in
-    let mi' = {leaf_credential=c.leaf_credential; leaf_version=1} in
-    (match update_path l t 0 mi' with
-    | None -> None
-    | Some p -> let t' = apply_path l 0 c.leaf_credential t p in
-		   let g0 = {st_group_id=gid;
-                   st_levels=l;
-			          st_tree=t';
-                   st_epoch=0;
-			          st_transcript_hash = empty} in
-		   let h0 = hash_state g0 in
-		   Some ({g0 with st_transcript_hash = h0}))
-
-val leaf_init: oc:option (c:credential_t) ->
-  om:option leaf_package_t{
-		      match oc,om with
-		      | None,None -> True
-		      | Some c,Some m -> m.leaf_credential == c
-		      | _ -> False}
-
-let leaf_init oc =
-  match oc with
-  | None -> None
-  | Some c -> Some ({leaf_credential = c; leaf_version = 0})
-
-val leaf_updated: sz:nat -> i:nat{i < sz} -> member_array_t sz -> member_array_t sz -> Type0
-let leaf_updated sz i m1 m2 =
-  match m1.[i] with
-  | None -> False
-  | Some mi -> (exists mi'. m2 == (m1.[i] <- Some mi') /\ name(mi'.leaf_credential) == name(mi.leaf_credential))
-
-val create_lemma: gid:nat -> sz:pos -> init:member_array_t sz
-	-> entropy:bytes_t	-> Lemma(
-	     match create gid sz init entropy with
-	     | None -> True
-	     | Some g ->
-		    group_id g == gid /\  max_size g == sz /\ epoch g == 0 /\
-		    leaf_updated sz 0 init (membership g))
-
-let create_lemma gid sz init leaf_secret =
-  match init.[0], log2 sz with
-  | None,_ -> ()
-  | _,None -> ()
-  | Some c,Some l ->
-    let t = create_tree l c.leaf_credential init in
-    let lp' = {leaf_credential = c.leaf_credential; leaf_version = 1} in
-    (match update_path l t 0 lp' with
-    | None -> ()
-    | Some p -> (update_path_lemma l 0 c.leaf_credential t lp';
-		   let t' = apply_path l 0 c.leaf_credential t p in
-		   assert (membership_tree l t == init);
-		   assert (membership_tree l t' == ((membership_tree  l t).[0] <- Some lp'));
-		   assert (leaf_updated sz 0 (membership_tree l t) (membership_tree l t'))))
-
-
-type operation_t : eqtype= {
-  op_level: nat;
-  op_index: index_n op_level;
-  op_actor: credential_t;
-  op_path: path_t op_level & path_t op_level
-}
-
-
-assume val hash_op: bytes_t -> operation_t -> bytes_t
+  | _ -> None
+  | Some actor,Some l ->
+    let t = create_tree l actor init in
+    let lp = {leaf_credential = actor;
+              leaf_version = 1; leaf_content = empty_bytes} in
+	 let st0 = {st_group_id = gid; st_levels = l;
+			     st_tree = t; st_version = 0;
+			     st_transcript = empty} in
+	 Some ({st0 with st_transcript = empty_bytes})
 
 
 (* Apply an operation to a state *)
-val apply: state_t -> operation_t -> option state_t
-let apply g o =
-  if o.op_level <> g.st_levels then None
-  else let p1,p2 = o.op_path in
-       let t' = apply_path o.op_level o.op_index o.op_actor g.st_tree p1 in
-       let t' = apply_path o.op_level o.op_index o.op_actor g.st_tree p2 in
-       Some ({g with st_epoch = g.st_epoch + 1; st_tree = t';
-  	     st_transcript_hash = hash_op g.st_transcript_hash o})
+val apply: state_t -> operation_t
+  -> Tot (option state_t)
 
-let update_leaf_package (lp:leaf_package_t) (nc:credential_t) = {
-  lp with
-  leaf_version = lp.leaf_version + 1;
-  leaf_credential = nc
-}
+let apply st op =
+  if op.op_level <> st.st_levels then None
+  else
+    let nt = apply_path op.op_level op.op_index op.op_actor st.st_tree op.op_path in
+    Some ({st with st_version = st.st_version + 1; st_tree = nt;
+  	                st_transcript = st.st_transcript})
 
-(* Create an operation that modifies the group state *)
-val modify: s:state_t -> actor:index_t s
-	-> i:index_t s -> option leaf_package_t
-	-> option operation_t
 
-let modify g actor i olp =
-  match (membership g).[actor] with
-  | None -> None
-  | Some mi_a_old ->
-    match olp with
-    | None -> None
-    | Some lp ->
-      let mi_a = update_leaf_package mi_a_old lp.leaf_credential in
-      let bp = blank_path g.st_levels i olp in
-      let nt = apply_path g.st_levels i mi_a.leaf_credential g.st_tree bp in
-      match update_path g.st_levels nt i mi_a with
-      | None -> None
-      | Some up -> Some ({op_level = g.st_levels; op_actor=mi_a.leaf_credential;
-	                     op_index = i; op_path = (bp,up)})
+
+
+
+
+val add: st:state_t -> actor:credential_t
+  -> i:index_t st -> joiner:credential_t
+  -> Tot (option (operation_t & state_t))
+
+
+val remove: st:state_t -> actor:credential_t -> i:index_t st
+  -> Tot (option (operation_t & state_t))
+
+
+
+// Construct operation
+// Precondition guarantees that you cannot change the membership
+// Only provide keypackages from the leaf to the root.
+
+
+
+/// Are we missing an extend operation for the tree?
+
+
+(* let update_leaf_package (lp:leaf_package_t) (nc:credential_t) = { *)
+(*   lp with *)
+(*   leaf_version = lp.leaf_version + 1; *)
+(*   leaf_credential = nc *)
+(* } *)
+
+
+
+
+// TODO: Signature
+
+
+
+// If 2 principals have consistent transcript => Group State is the same.
+// Signatures: if the last actor is honest the transcript of the sender and recipients are the same = consistent
+
