fstar/new/Lib.Array.fst
@@ -1,0 +1,55 @@
+module Lib.Array
+
+(* Datastructures *)
+let array a = Seq.seq a
+let length a = Seq.length a
+let empty = Seq.empty
+let singleton x = Seq.create 1 x
+let append x y = Seq.append x y
+
+(* Infix operators *)
+let op_String_Access x y = Seq.index x y
+let op_String_Assignment x y z = Seq.upd x y z
+
+(* Datastructures operators *)
+let rec mapi (f:'a -> 'b) (x:array 'a) (i:nat{i <= length x}) : y:array 'b{length y = i} =
+  if i = 0 then empty else Seq.snoc (mapi f x (i-1)) (f x.[i-1])
+
+let map (f:'a -> 'b) (x:array 'a) = mapi f x (length x)
+
+
+val lemma_singleton: x:array 'a{length x = 1} -> i:nat{i<length x} ->
+  Lemma (singleton x.[i] == x)
+	[SMTPat (singleton x.[i])]
+let lemma_singleton x i = Seq.lemma_eq_intro (singleton x.[i]) x
+
+val lemma_map_singleton: f:('a -> 'b) -> x:array 'a{length x = 1} ->
+    Lemma (singleton (f (x.[0])) == map f x)
+	  [SMTPatOr [
+	    [SMTPat (singleton (f (x.[0])));
+	     SMTPat (map f x)]]]
+let lemma_map_singleton f x = admit()
+
+val lemma_map_append: f:('a -> 'b) -> x:array 'a -> y:array 'a ->
+    Lemma (append (map f x) (map f y) == map f (append x y))
+	  [SMTPatOr [
+	    [SMTPat (append (map f x) (map f y));
+	     SMTPat (map f (append x y))]]]
+let lemma_map_append f x y = admit()
+
+
+let sub (x:array 'a) (i:nat{i < length x}) (l:nat{i+l <= length x}) = Seq.slice x i (i+l)
+
+let split (x:array 'a) (i:nat{i < length x}): res:(array 'a * array 'a){let (y,z) = res in x == append y z /\ length y = i} =
+  let s1 = sub x 0 i in
+  let s2 = sub x i (length x - i) in
+  Seq.lemma_eq_intro x (append s1 s2);
+  (s1,s2)
+
+
+let rec foldi (f:'a -> 'b -> 'a) (x:array 'b) (init:'a) (n:nat{n <= length x}) =
+  if n = 0 then init
+  else f (foldi f x init (n-1)) x.[n-1]
+
+val fold: f:('a -> 'b -> 'a) -> array 'b -> 'a -> 'a
+let fold f x a = foldi f x a (length x)
