fstar/new/TreeSync.Lemmas.fst
@@ -1,0 +1,35 @@
+module TreeSync.Lemmas
+
+open Lib.Array
+open TreeSync
+
+let rec blank_path_lemma (l:nat) (i:index_n l) (olp:option credential_t) (a:credential_t) (t:tree_t l) :
+                    Lemma (let t' = apply_path l i a t (blank_path l i olp) in
+                          membership_tree l t' == ((membership_tree l t).[i] <- olp)) =
+    match t with
+    | Leaf _ _ ->
+	   let t' = apply_path l i a t (blank_path l i olp) in
+	   Seq.lemma_eq_intro (membership_tree l t') ((membership_tree l t).[i] <- olp)
+    | Node _ _ left right ->
+      let (j,dir) = child_index l i in
+      let (child,sibling) = order_subtrees dir (left,right) in
+      let p = PNode None (blank_path (l-1) j olp) in
+      blank_path_lemma (l-1) j olp a child;
+      let t' = apply_path l i a t (blank_path l i olp) in
+      Seq.lemma_eq_intro (membership_tree l t') ((membership_tree l t).[i] <- olp)
+
+
+val mk_operation_lemma: st:state_t -> actor:credential_t
+  -> i:index_t st -> p:path_t st.st_levels
+  -> Tot (oop:option operation_t{
+         match oop with
+         | None -> True
+         | Some op ->
+         match apply st op with
+         | None -> False
+		   | Some st' -> group_id st' == group_id st
+  		              /\ max_size st' == max_size st
+			           /\ epoch st' == epoch st + 1
+			           /\ (match op.op_path with
+                      | PLeaf olp -> membership st' == membership st
+                      | _ -> True)})
